HoareLogic/SequentialSemantics.v
@@ -1,0 +1,27 @@
+Require Import Logic.MinimunLogic.LogicBase.
+Require Import Logic.SeparationLogic.SeparationAlgebra.
+Require Import Logic.HoareLogic.ImperativeLanguage.
+
+Inductive MetaState (state: Type): Type :=
+  | Error: MetaState state
+  | NonTerminating: MetaState state
+  | Terminating: state -> MetaState state.
+
+Arguments Error {_}.
+Arguments NonTerminating {_}.
+Arguments Terminating {_} _.
+
+Class BigStepSemantics (P: ProgrammingLanguage) (state: Type): Type := {
+  access: state -> cmd -> MetaState state -> Prop
+}.
+
+Definition safe {P: ProgrammingLanguage} {state: Type} {BSS: BigStepSemantics P state} (s: state) (c: cmd): Prop :=
+  ~ access s c Error.
+
+Definition term_norm {P: ProgrammingLanguage} {state: Type} {BSS: BigStepSemantics P state} (s: state) (c: cmd): Prop :=
+  ~ access s c Error /\ ~ access s c NonTerminating.
+
+Class NormalBigStepSemantics (P: ProgrammingLanguage) (state: Type) (BSS: BigStepSemantics P state): Type := {
+  access_defined: forall s c, exists ms, access s c ms
+}.
+
